\documentclass[a4paper,10pt,fleqn]{scrartcl}

\usepackage{amsmath}
\usepackage{mathtools}
\usepackage{amssymb}
\usepackage{a4wide}
\usepackage{subcaption}
\usepackage{dsfont}
\usepackage[utf8x]{inputenc}

\newcommand{\xpFq}[2]{{{}_{#1} F_{#2}}}
\newcommand{\pFq}[5]{{\xpFq{#1}{#2}\left(\begin{matrix} {#3} \\ {#4} \end{matrix} \middle| {#5}\right)}}

\parindent0pt

\begin{document}

    \begin{align*}
        0
        &=
        \sum_{n=0}^{\hat n}
        p_n(x)
        \frac{\partial^n}{\partial x^n}
        \Psi(x) \\
        p_n(x)
        &=
        \sum_{m=0}^{\hat m}
        p_{nm}
        x^m
    \end{align*}

    \begin{align*}
        \Psi(x+\delta)
        &=
        \sum_{k=k_0}^\infty a_k(\Psi;x)\delta^{k/2}
    \end{align*}

    \begin{align*}
        0
        &=
        \sum_{n=0}^{\hat n}
        p_n(x+\delta)
        \frac{\partial^n}{\partial \delta^n}
        \Psi(x+\delta)
        \\
        &=
        \sum_{n=0}^{\hat n}
        \sum_{m=0}^{\hat m}
        p_{nm} (x+\delta)^m
        \frac{\partial^n}{\partial \delta^n}
        \Psi(x+\delta)
        \\
        &=
        \sum_{n=0}^{\hat n}
        \sum_{m=0}^{\hat m}
        \sum_{j=0}^m
        \binom{m}{j}
        p_{nm} x^{m-j}
        \delta^j
        \frac{\partial^n}{\partial \delta^n}
        \Psi(x+\delta)
    \end{align*}

    \begin{align*}
        0
        &=
        \sum_{n=0}^{\hat n}
        \sum_{m=0}^{\hat m}
        \sum_{j=0}^m
        \sum_{k=k_0}^\infty
        \binom{m}{j}
        a_k(\Psi;x)
        p_{nm} x^{m-j}
        \delta^j
        \frac{\partial^n}{\partial \delta^n}
        \delta^{k/2}
        \\
        &=
        \sum_{n=0}^{\hat n}
        \sum_{m=0}^{\hat m}
        \sum_{j=0}^m
        \sum_{k=k_0}^\infty
        (-1)^n
        (-k/2)_n
        \binom{m}{j}
        a_k(\Psi;x)
        p_{nm} x^{m-j}
        \delta^{j+k/2-n}
        \\
        &=
        \sum_{n=0}^{\hat n}
        \sum_{m=0}^{\hat m}
        \sum_{j=0}^m
        \sum_{k=k_0+2j-2n}^\infty
        (-1)^n
        (-k/2+j-n)_n
        \binom{m}{j}
        a_{k-2j+2n}(\Psi;x)
        p_{nm} x^{m-j}
        \delta^{k/2}
        \\
        &=
        \sum_{n=0}^{\hat n}
        \sum_{k=k0-2n}^\infty
        \sum_{m=0}^{\hat m}
        \hspace{-3pt}
        \sum_{j=0}^{\min\left(m,n+\lfloor (k-k_0)/2 \rfloor\right)}
        \hspace{-10pt}
        (-1)^n
        (-k/2+j-n)_n
        \binom{m}{j}
        a_{k-2j+2n}(\Psi;x)
        p_{nm} x^{m-j}
        \delta^{k/2}
        \\
        &=
        \sum_{k=k0-2\hat n}^\infty
        \sum_{n=\max\left(0,\lceil (k_0-k)/2 \rceil\right)}^{\hat n}
        \sum_{m=0}^{\hat m}
        \hspace{-3pt}
        \sum_{j=0}^{\min\left(m,n+\lfloor (k-k_0)/2 \rfloor\right)}
        \hspace{-10pt}
        (-1)^n
        (-k/2+j-n)_n
        \binom{m}{j}
        a_{k-2j+2n}(\Psi;x)
        p_{nm} x^{m-j}
        \delta^{k/2}
    \end{align*}

    \begin{align*}
        0
        &=
        \sum_{n=\max\left(0,\lceil (k_0-k)/2 \rceil\right)}^{\hat n}
        \sum_{m=0}^{\hat m}
        \hspace{-3pt}
        \sum_{j=0}^{\min\left(m,n+\lfloor (k-k_0)/2 \rfloor\right)}
        \hspace{-10pt}
        (-1)^n
        (-k/2+j-n)_n
        \binom{m}{j}
        a_{k-2j+2n}(\Psi;x)
        p_{nm} x^{m-j}
        \\
        &=
        \sum_{n=\max\left(0,\lceil (k_0-k)/2 \rceil\right)}^{\hat n}
        \sum_{m=0}^{\hat m}
        \hspace{-3pt}
        \sum_{j=-n}^{\min\left(m-n,\lfloor (k-k_0)/2 \rfloor\right)}
        \hspace{-10pt}
        (-1)^n
        (-k/2+j)_n
        \binom{m}{j+n}
        a_{k-2j}(\Psi;x)
        p_{nm} x^{m-j-n}
        \\
        &=
        \sum_{n=\max\left(0,\lceil (k_0-k)/2 \rceil\right)}^{\hat n}
        \sum_{m=0}^{\hat m}
        \hspace{-3pt}
        \sum_{j=-n}^{\min\left(m-n,\lfloor (k-k_0)/2 \rfloor\right)}
        \hspace{-10pt}
        (-1)^n
        (-k/2+j)_n
        \binom{m}{j+n}
        a_{k-2j}(\Psi;x)
        p_{nm} x^{m-j-n}
        \\
        &=
        \sum_{n=\max\left(0,\lceil (k_0-k)/2 \rceil\right)}^{\hat n}
        \hspace{-3pt}
        \sum_{j=-n}^{\min\left(\hat m-n,\lfloor (k-k_0)/2 \rfloor\right)}
        \hspace{-10pt}
        \sum_{m=j+n}^{\hat m}
        (-1)^n
        (-k/2+j)_n
        \binom{m}{j+n}
        a_{k-2j}(\Psi;x)
        p_{nm} x^{m-j-n}
        \\
        &=
        \sum_{j=-\hat n}^{\min\left(\hat m,\lfloor (k-k_0)/2 \rfloor\right)}
        \sum_{n=\max(0,-j)}^{\min(\hat n,\hat m-j)}
        \sum_{m=j+n}^{\hat m}
        (-1)^n
        (-k/2+j)_n
        \binom{m}{j+n}
        a_{k-2j}(\Psi;x)
        p_{nm} x^{m-j-n}
        \\
        &=
        \sum_{j=\max\left(-\hat m,\lceil (k_0-k)/2 \rceil\right)}^{\hat n}
        \sum_{n=\max(0,j)}^{\min(\hat n,\hat m+j)}
        \sum_{m=n-j}^{\hat m}
        (-1)^n
        (-k/2-j)_n
        \binom{m}{n-j}
        a_{k+2j}(\Psi;x)
        p_{nm} x^{m+j-n}
        \\
        &=
        \sum_{j=\max\left(-\hat m,\lceil (k_0-k)/2 \rceil\right)}^{\hat n}
        \sum_{n=\max(0,j)}^{\min(\hat n,\hat m+j)}
        \frac{(-1)^n(-k/2-j)_n}{(n-j)!}
        a_{k+2j}(\Psi;x)
        \sum_{m=n-j}^{\hat m}
        \frac{m!}{(m+j-n)!}
        p_{nm} x^{m+j-n}
        \\
        &=
        \sum_{j=\max\left(-\hat m,\lceil (k_0-k)/2 \rceil\right)}^{\hat n}
        a_{k+2j}(\Psi;x)
        \sum_{n=\max(0,j)}^{\min(\hat n,\hat m+j)}
        \frac{(-1)^n(-k/2-j)_n}{(n-j)!}
        p^{(n-j)}_n(x)
        \\
        &=
        \sum_{j=\max\left(-\hat m,\lceil (k_0-k)/2 \rceil\right)}^{\hat n}
        a_{k+2j}(\Psi;x)
        C_{jk}(x)
    \end{align*}

    \begin{align*}
        C_{jk}(x)
        &=
        \sum_{n=\max(0,j)}^{\min(\hat n,\hat m+j)}
        \frac{(-1)^n(-k/2-j)_n}{(n-j)!}
        p^{(n-j)}_n(x)
    \end{align*}


    \begin{align*}
        C_{jk}(x)
        &=
        0
        \quad;\quad
        j > \hat n-r \\
        C_{\hat n-r,k} &\neq 0
    \end{align*}

    \begin{align*}
        a_{k+2\hat n-2r}(\Psi;x)
        C_{\hat n-r,k}(x)
        &=
        -
        \sum_{j=\max\left(-\hat m,\lceil (k_0-k)/2 \rceil\right)}^{\hat n-r-1}
        a_{k+2j}(\Psi;x)
        C_{jk}(x)
        \\
        a_{k+2\hat n-2r}(\Psi;x)
        &=
        -
        \frac1{C_{\hat n-r,k}(x)}
        \sum_{j=\max\left(-\hat m,\lceil (k_0-k)/2 \rceil\right)}^{\hat n-r-1}
        a_{k+2j}(\Psi;x)
        C_{jk}(x)
        \\
        a_k(\Psi;x)
        &=
        -
        \frac1{C_{\hat n-r,k-2\hat n+2r}(x)}
        \sum_{j=\max\left(-\hat m,\lceil (k_0-k)/2 \rceil+\hat n-r\right)}^{\hat n-r-1}
        a_{k-2\hat n+2r+2j}(\Psi;x)
        C_{j,k-2\hat n+2r}(x)
    \end{align*}
\end{document}
