\documentclass[a4paper,10pt,fleqn]{scrartcl}

\usepackage{amsmath}
\usepackage{mathtools}
\usepackage{amssymb}
\usepackage{a4wide}
\usepackage{subcaption}
\usepackage{dsfont}
\usepackage[utf8x]{inputenc}

\newcommand{\xpFq}[2]{{{}_{#1} F_{#2}}}
\newcommand{\pFq}[5]{{\xpFq{#1}{#2}\left(\begin{matrix} {#3} \\ {#4} \end{matrix} \middle| {#5}\right)}}

\parindent0pt

\begin{document}
    \begin{align*}
        f(x) &= \sum\limits_{n=n_0}^\infty a_n x^n \\
        \frac1{f(x)} &= \sum\limits_{k=-n_0}^\infty b_k x^k
    \end{align*}

    \begin{align*}
        1
        &=
        f(x) \times \frac1{f(x)}
        \\
        &=
        \sum\limits_{n=n_0}^\infty
        \sum\limits_{k=-n_0}^\infty
        a_n
        b_k
        x^{n+k}
        \\
        &=
        \sum\limits_{n=n_0}^\infty
        \sum\limits_{k=n-n_0}^\infty
        a_n
        b_{k-n}
        x^k
        \\
        &=
        \sum\limits_{n=n_0}^\infty
        \sum\limits_{k=n-n_0}^\infty
        a_n
        b_{k-n}
        x^k
        \\
        &=
        \sum\limits_{k=0}^\infty
        x^k
        \sum\limits_{n=n_0}^{n_0+k}
        a_n
        b_{k-n}
        \\
        &=
        \sum\limits_{k=0}^\infty
        x^k
        \sum\limits_{n=0}^{k}
        a_{n+n_0}
        b_{k-n-n_0}
    \end{align*}

    \begin{align*}
        \sum\limits_{n=0}^{k}
        a_{n+n_0}
        b_{k-n-n_0}
        &=
        \delta_{k0}
    \end{align*}

    \begin{align*}
        a_{n_0}
        b_{-n_0}
        &=
        1
        \quad\Rightarrow\quad
        b_{-n_0} = \frac1{a_{n_0}}
    \end{align*}

    \begin{align*}
        a_{n_0}
        b_{k-n_0}
        &=
        -
        \sum\limits_{n=1}^{k}
        a_{n+n_0}
        b_{k-n-n_0}
        \\
        b_{k-n_0}
        &=
        -
        \frac1{a_{n_0}}
        \sum\limits_{n=1}^{k}
        a_{n+n_0}
        b_{k-n-n_0}
    \end{align*}

    \begin{align*}
        b_{-n_0} &= \frac1{a_{n_0}} \\
        b_{k}
        &=
        -
        \frac1{a_{n_0}}
        \sum\limits_{n=1}^{k+n_0}
        a_{n+n_0}
        b_{k-n}
        \quad;\quad k>-n_0
    \end{align*}

\end{document}
