\documentclass[a4paper,10pt,fleqn]{scrartcl}

\usepackage{amsmath}
\usepackage{mathtools}
\usepackage{amssymb}
\usepackage{a4wide}
\usepackage{subcaption}
\usepackage{dsfont}
\usepackage[utf8x]{inputenc}

\newcommand{\xpFq}[2]{{{}_{#1} F_{#2}}}
\newcommand{\pFq}[5]{{\xpFq{#1}{#2}\left(\begin{matrix} {#3} \\ {#4} \end{matrix} \middle| {#5}\right)}}

\parindent0pt

\begin{document}
    \begin{align*}
        I(f_1,\cdots,f_N;x)
        &=
        \int\limits_0^{x} \mathrm{d}t\,f_1(t) I(f_2,\cdots,f_N;t)
    \end{align*}

    \begin{align*}
        I(f_1,\cdots,f_N;x+\delta)
        &=
        \sum\limits_{n=0}^\infty
        \sum\limits_{m=0}^\infty
        c_{nm}(f_1,\cdots,f_N;x)
        \delta^{n/2}
        \ln^m(\delta)
        \\
        f_j(x+\delta)
        &=
        \sum\limits_{k=k_0}^\infty
        a_k(f_j;x)
        \delta^{k/2}
    \end{align*}

    \begin{align*}
        I(f_1,\cdots,f_N;x+\delta)
        &=
        \int\limits_0^{x+\delta} \mathrm{d}t\,f_1(t) I(f_2,\cdots,f_N;t)
        \\
        &=
        \int\limits_{-x}^{\delta} \mathrm{d}\Delta\,f_1(x+\Delta) I(f_2,\cdots,f_N;x+\Delta)
        \\
        &=
        {\tilde I}(f_1,\cdots,f_N;x)
        +
        \int\limits^{\delta} \mathrm{d}\Delta\,f_1(x+\Delta) I(f_2,\cdots,f_N;x+\Delta)
        \\
        &=
        {\tilde I}(f_1,\cdots,f_N;x)
        \\ &\quad
        +
        \sum\limits_{k=k_0}^\infty
        \sum\limits_{n=0}^\infty
        \sum\limits_{m=0}^\infty
        a_k(f_1;x)
        c_{nm}(f_2,\cdots,f_N;x)
        \int\limits^{\delta} \mathrm{d}\Delta\,
        \Delta^{(k+n)/2}
        \ln^m(\Delta)
        \\
        &=
        {\tilde I}(f_1,\cdots,f_N;x)
        \\ &\quad
        +
        \sum\limits_{n=k_0}^\infty
        \sum\limits_{m=0}^\infty
        \int\limits^{\delta} \mathrm{d}\Delta\,
        \Delta^{n/2}
        \ln^m(\Delta)
        \sum\limits_{k=k_0}^n
        a_k(f_1;x)
        c_{n-k,m}(f_2,\cdots,f_N;x)
        \\
        %%%%%%%%%%%%%%%%%%%%%%%%%%%%%%%%%%%%%%%
        &=
        {\tilde I}(f_1,\cdots,f_N;x)
        \\ &\quad
        +
        \sum_{\substack{n=k_0\\n\neq-2}}^\infty
        \sum_{m=0}^\infty
        \int\limits^{\delta} \mathrm{d}\Delta\,
        \Delta^{n/2}
        \ln^m(\Delta)
        \sum\limits_{k=k_0}^n
        a_k(f_1;x)
        c_{n-k,m}(f_2,\cdots,f_N;x)
        \\ &\quad
        +
        \sum_{m=0}^\infty
        \int\limits^\delta \mathrm{d}\Delta\,
        \frac{\ln^m(\Delta)}{\Delta}
        \sum\limits_{k=k_0}^{-2}
        a_k(f_1;x)
        c_{-2-k,m}(f_2,\cdots,f_N;x)
        \\
        %%%%%%%%%%%%%%%%%%%%%%%%%%%%%%%%%%%%%%%
        &=
        {\tilde I}(f_1,\cdots,f_N;x)
        \\ &\quad
        -
        \sum_{\substack{n=k_0\\n\neq-2}}^\infty
        \sum_{m=0}^\infty
        \sum\limits_{j=0}^m
        \delta^{n/2+1}
        \ln^j(\delta)
        \frac{m!\,(-1-n/2)^{j-m-1}}{j!}
        \sum\limits_{k=k_0}^n
        a_k(f_1;x)
        c_{n-k,m}(f_2,\cdots,f_N;x)
        \\ &\quad
        +
        \sum_{m=0}^\infty
        \frac{\ln^{m+1}(\delta)}{m+1}
        \sum\limits_{k=k_0}^{-2}
        a_k(f_1;x)
        c_{-2-k,m}(f_2,\cdots,f_N;x)
        \\
        %%%%%%%%%%%%%%%%%%%%%%%%%%%%%%%%%%%%%%%
        &=
        {\tilde I}(f_1,\cdots,f_N;x)
        \\ &\quad
        -
        \sum_{\substack{n=k_0\\n\neq-2}}^\infty
        \sum_{j=0}^\infty
        \delta^{n/2+1}
        \ln^j(\delta)
        \sum_{m=j}^\infty
        \sum\limits_{k=k_0}^n
        \frac{m!\,(-1-n/2)^{j-m-1}}{j!}
        a_k(f_1;x)
        c_{n-k,m}(f_2,\cdots,f_N;x)
        \\ &\quad
        +
        \sum_{m=0}^\infty
        \frac{\ln^{m+1}(\delta)}{m+1}
        \sum\limits_{k=k_0}^{-2}
        a_k(f_1;x)
        c_{-2-k,m}(f_2,\cdots,f_N;x)
        \\
        %%%%%%%%%%%%%%%%%%%%%%%%%%%%%%%%%%%%%%%
        &=
        {\tilde I}(f_1,\cdots,f_N;x)
        \\ &\quad
        -
        \sum_{\substack{n=k_0+2\\n\neq0}}^\infty
        \sum_{j=0}^\infty
        \delta^{n/2}
        \ln^j(\delta)
        \sum_{m=j}^\infty
        \sum\limits_{k=k_0}^{n-2}
        \frac{m!\,(-n/2)^{j-m-1}}{j!}
        a_k(f_1;x)
        c_{n-k-2,m}(f_2,\cdots,f_N;x)
        \\ &\quad
        +
        \sum_{m=1}^\infty
        \frac{\ln^m(\delta)}{m}
        \sum\limits_{k=k_0}^{-2}
        a_k(f_1;x)
        c_{-2-k,m-1}(f_2,\cdots,f_N;x)
    \end{align*}

    \begin{align*}
        c_{00}
        &=
        {\tilde I}(f_1,\cdots,f_N;x)
        \\
        c_{0,m>0}
        &=
        \frac{\ln^m(\delta)}{m}
        \sum\limits_{k=k_0}^{-2}
        a_k(f_1;x)
        c_{-2-k,m-1}(f_2,\cdots,f_N;x)
        \\
        c_{n\neq 0,j}
        &=
        -
        \sum_{m=j}^\infty
        \sum\limits_{k=k_0}^{n-2}
        \frac{m!\,(-n/2)^{j-m-1}}{j!}
        a_k(f_1;x)
        c_{n-k-2,m}(f_2,\cdots,f_N;x)
    \end{align*}

    \appendix
    \section{auxiliary integrals}
    \begin{align*}
        \int\limits^\delta \mathrm{d}\Delta\,
        \Delta^{n/2}
        \ln^m(\Delta)
        &=
        -m!\,
        \delta^{n/2+1}
        \sum\limits_{j=0}^m
        \frac{(-1-n/2)^{j-m-1}}{j!}
        \ln^j(\delta)
        \quad;\quad n\neq-2
        \\
        \int\limits^{\delta} \mathrm{d}\Delta\,
        \frac{\ln^m(\Delta)}{\Delta}
        &=
        \frac{\ln^{m+1}(\delta)}{m+1}
    \end{align*}
\end{document}
